\input{header.tex}

\title{Bernstein-concentration}

\begin{document}

\maketitle
\initMinimal{}

\begin{definition}[$\gamma$-bernstein-concentration]
A random variable $X \in \mathbb{R}^n$ is $\gamma$-bernstein-concentrated iff
\[ \Pr[a^TX - \E(a^TX) \ge t]
\le \exp\left( \frac{-1}{2\gamma} \; \frac{t^2}{\sum_{i=1}^n a_i^2 \Var(X_i) + \frac{Mt}{3}} \right) \]
where $M = \max_{i=1}^n \abs{a_i(X_i - \E(X_i))}$.
\end{definition}

\begin{theorem}[Bernstein's inequality]
Let $X \in \mathbb{R}^n$ be a random variable where each coordinate of $X$ is independent.
Then $X$ is $1$-bernstein-concentrated.
\end{theorem}

\section{Bernouilli variables}

\begin{theorem}
\label{thm:refined-bern-conc}
Let $X \in \{0, 1\}^n$ be a random variable with $\E(X) = x$.
If $X$ is $\gamma$-bernstein-concentrated, then
\[ \Pr[a^TX - a^Tx \ge t]
\le \exp\left( \frac{-1}{2\gamma} \; \frac{t^2}{\norm{a}_{\infty}(a^Tx + t/3)} \right) \]
\end{theorem}
\begin{proof}
$\Var(X_i) = x_i(1-x_i)$.
\[ \sum_{i=1}^n a_i^2 x_i(1-x_i)
\le \norm{a}_{\infty} \sum_{i=1}^n a_ix_i
= \norm{a}_{\infty} a^Tx \]
\[ M = \max_{i=1}^n \abs{a_i}\abs{X_i - \E(X_i)}
\le \norm{a}_{\infty} \max_{i=1}^n \abs{X_i - \E(X_i)}
\le \norm{a}_{\infty} \]
\end{proof}

\begin{theorem}
Let $X \in \{0, 1\}^n$ be a random variable with $\E(X) = x$.
Let $X$ be $\gamma$-bernstein-concentrated.
Let $\alpha \le a^Tx \le \beta$. Then
\[ \Pr[ a^TX \ge (1+\delta)\beta ]
\le \exp\left(\frac{-1}{2\gamma} \frac{\beta}{\norm{a}_{\infty}} \frac{\delta^2}{1+\delta/3} \right) \]
\[ \Pr[ a^TX \le (1-\delta)\alpha ]
\le \exp\left(\frac{-1}{2\gamma} \frac{\alpha}{\norm{a}_{\infty}} \frac{\delta^2}{1+\delta/3} \right) \]
\end{theorem}
\begin{proof}
Let $c = (1+\delta)\beta$.
\begin{align*}
\Pr[ a^TX \ge c ]
&= \Pr[ a^TX - a^Tx \ge c - a^Tx ]
\\ &\le \exp\left( -\frac{1}{2\gamma} \; \frac{(c-a^Tx)^2}{\norm{a}_{\infty}
\left(a^Tx + \frac{1}{3}(c - a^Tx)\right)} \right)
\tag{by theorem \ref{thm:refined-bern-conc}}
\\ &\le \exp\left( -\frac{1}{2\gamma} \frac{3}{\norm{a}_{\infty}} \frac{(c-a^Tx)^2}{c + 2a^Tx} \right)
\end{align*}
Let $f(y) = (c-y)^2/(c+2y)$, where $y \in [\alpha, \beta]$. $f(y) > 0$.
\[ \ln(f(y)) = 2\ln(c-y) - \ln(c+2y) \]
\[ \frac{f'(y)}{f(y)} = -\frac{2}{c-y} - \frac{2}{c+2y} < 0 \]
Since $f'(y) < 0$, $f(y)$ is minimized at $y = \beta$.
$f(\beta) = (\delta^2\beta)/(3 + \delta)$.
Therefore,
\[ \Pr[ a^TX \ge (1+\delta)\beta ]
\le \exp\left( \frac{-1}{2\gamma} \frac{\beta}{\norm{a}_{\infty}} \frac{\delta^2}{1+\delta/3} \right) \]
The other inequality can be proven similarly.
\end{proof}

%\addMyBib{}

\end{document}
